Bridge direct receiver safety gate

rocq/theories/TypeSystem/EnvRuntimeCapturedSafety.v
@@ -15622,6 +15622,119 @@ Proof.
   - eapply Hbody_replay_consumed; eassumption.
 Qed.
 
+
+Definition direct_receiver_method_live_raw_body_replay_provider_for_eval
+    (env : global_env) (fdef : fn_def) (s s' : store) (v : value)
+    : Prop :=
+  forall method_name type_args receiver_name receiver_args method_args
+      receiver_callee method_callee,
+    (exists s_receiver_raw v_receiver_raw s_args_raw vs_method_raw
+        fcall_raw used_raw s_body_raw,
+      eval (global_env_with_local_bounds env (fn_bounds fdef))
+        s (ECall receiver_name receiver_args) s_receiver_raw
+        v_receiver_raw /\
+      eval_args (global_env_with_local_bounds env (fn_bounds fdef))
+        s_receiver_raw method_args s_args_raw vs_method_raw /\
+      lookup_fn method_name
+        (env_fns (global_env_with_local_bounds env (fn_bounds fdef))) =
+        Some method_callee /\
+      fn_captures method_callee = [] /\
+      alpha_rename_fn_def (store_names s_args_raw) method_callee =
+        (fcall_raw, used_raw) /\
+      eval (global_env_with_local_bounds env (fn_bounds fdef))
+        (bind_params (apply_type_params type_args (fn_params fcall_raw))
+          (v_receiver_raw :: vs_method_raw) s_args_raw)
+        (subst_type_params_expr type_args (fn_body fcall_raw))
+        s_body_raw v /\
+      s' = store_remove_params
+        (apply_type_params type_args (fn_params fcall_raw)) s_body_raw) ->
+    forall s_receiver v_receiver,
+    eval (global_env_with_local_bounds env (fn_bounds fdef))
+      s (ECall receiver_name receiver_args) s_receiver v_receiver ->
+    forall s_args_base vs_method fcall_base used_base s_body_base,
+    eval_args (global_env_with_local_bounds env (fn_bounds fdef))
+      s_receiver method_args s_args_base vs_method ->
+    alpha_rename_fn_def (store_names s_args_base) method_callee =
+      (fcall_base, used_base) ->
+    eval (global_env_with_local_bounds env (fn_bounds fdef))
+      (bind_params (apply_type_params type_args (fn_params fcall_base))
+        (v_receiver :: vs_method) s_args_base)
+      (subst_type_params_expr type_args (fn_body fcall_base))
+      s_body_base v ->
+    forall s_var_hidden s_args_hidden,
+    eval (global_env_with_local_bounds env (fn_bounds fdef))
+      (store_add receiver_method_hidden_receiver_name
+        (fn_ret receiver_callee) v_receiver s_receiver)
+      (EVar receiver_method_hidden_receiver_name) s_var_hidden v_receiver ->
+    eval_args (global_env_with_local_bounds env (fn_bounds fdef))
+      s_var_hidden method_args s_args_hidden vs_method ->
+    store_hidden_frame_rel receiver_method_hidden_receiver_name
+      (fn_ret receiver_callee) v_receiver s_args_hidden s_args_base ->
+    exists fcall_hidden used_hidden s_body_hidden,
+      alpha_rename_fn_def (store_names s_args_hidden) method_callee =
+        (fcall_hidden, used_hidden) /\
+      eval (global_env_with_local_bounds env (fn_bounds fdef))
+        (bind_params (apply_type_params type_args (fn_params fcall_hidden))
+          (v_receiver :: vs_method) s_args_hidden)
+        (subst_type_params_expr type_args (fn_body fcall_hidden))
+        s_body_hidden v.
+
+Definition direct_receiver_method_consumed_raw_body_replay_provider_for_eval
+    (env : global_env) (fdef : fn_def) (s s' : store) (v : value)
+    : Prop :=
+  forall method_name type_args receiver_name receiver_args method_args
+      receiver_callee method_callee,
+    (exists s_receiver_raw v_receiver_raw s_args_raw vs_method_raw
+        fcall_raw used_raw s_body_raw,
+      eval (global_env_with_local_bounds env (fn_bounds fdef))
+        s (ECall receiver_name receiver_args) s_receiver_raw
+        v_receiver_raw /\
+      eval_args (global_env_with_local_bounds env (fn_bounds fdef))
+        s_receiver_raw method_args s_args_raw vs_method_raw /\
+      lookup_fn method_name
+        (env_fns (global_env_with_local_bounds env (fn_bounds fdef))) =
+        Some method_callee /\
+      fn_captures method_callee = [] /\
+      alpha_rename_fn_def (store_names s_args_raw) method_callee =
+        (fcall_raw, used_raw) /\
+      eval (global_env_with_local_bounds env (fn_bounds fdef))
+        (bind_params (apply_type_params type_args (fn_params fcall_raw))
+          (v_receiver_raw :: vs_method_raw) s_args_raw)
+        (subst_type_params_expr type_args (fn_body fcall_raw))
+        s_body_raw v /\
+      s' = store_remove_params
+        (apply_type_params type_args (fn_params fcall_raw)) s_body_raw) ->
+    forall s_receiver v_receiver,
+    eval (global_env_with_local_bounds env (fn_bounds fdef))
+      s (ECall receiver_name receiver_args) s_receiver v_receiver ->
+    forall s_args_base vs_method fcall_base used_base s_body_base,
+    eval_args (global_env_with_local_bounds env (fn_bounds fdef))
+      s_receiver method_args s_args_base vs_method ->
+    alpha_rename_fn_def (store_names s_args_base) method_callee =
+      (fcall_base, used_base) ->
+    eval (global_env_with_local_bounds env (fn_bounds fdef))
+      (bind_params (apply_type_params type_args (fn_params fcall_base))
+        (v_receiver :: vs_method) s_args_base)
+      (subst_type_params_expr type_args (fn_body fcall_base))
+      s_body_base v ->
+    forall s_var_hidden s_args_hidden,
+    eval (global_env_with_local_bounds env (fn_bounds fdef))
+      (store_add receiver_method_hidden_receiver_name
+        (fn_ret receiver_callee) v_receiver s_receiver)
+      (EVar receiver_method_hidden_receiver_name) s_var_hidden v_receiver ->
+    eval_args (global_env_with_local_bounds env (fn_bounds fdef))
+      s_var_hidden method_args s_args_hidden vs_method ->
+    store_consumed_hidden_frame_rel receiver_method_hidden_receiver_name
+      (fn_ret receiver_callee) v_receiver s_args_hidden s_args_base ->
+    exists fcall_hidden used_hidden s_body_hidden,
+      alpha_rename_fn_def (store_names s_args_hidden) method_callee =
+        (fcall_hidden, used_hidden) /\
+      eval (global_env_with_local_bounds env (fn_bounds fdef))
+        (bind_params (apply_type_params type_args (fn_params fcall_hidden))
+          (v_receiver :: vs_method) s_args_hidden)
+        (subst_type_params_expr type_args (fn_body fcall_hidden))
+        s_body_hidden v.
+
 Lemma callee_body_root_shadow_captured_call_generic_direct_receiver_method_runtime_replay_checked_initial_branch_value :
   forall env fdef s s' v method_name type_args receiver_name
       receiver_type_args receiver_args method_args hidden_synthetic_body
@@ -21552,6 +21665,59 @@ Proof.
   - exact Hinitial.
   - exact Hstore.
   - exact Heval.
+Qed.
+
+
+Theorem callee_body_root_shadow_captured_call_store_safe_summary_with_direct_receiver_method_big_step_safe_checked_initial_ready_with_split_raw_body_replay :
+  forall env f s s' v,
+    fn_env_unique_by_name env ->
+    env_fns_root_shadow_provenance_summary_evidence env ->
+    env_fns_preservation_ready env ->
+    callee_body_root_shadow_captured_call_store_safe_summary_with_direct_receiver_method
+      env f ->
+    check_initial_root_runtime_ready f s = true ->
+    initial_store_for_fn env f s ->
+    eval env s (fn_body f) s' v ->
+    direct_receiver_method_live_raw_body_replay_provider_for_eval
+      env f s s' v ->
+    direct_receiver_method_consumed_raw_body_replay_provider_for_eval
+      env f s s' v ->
+    value_has_type env s' v (fn_ret f).
+Proof.
+  intros env f s s' v Hunique Hevidence Hready Hsummary Hinitial
+    Hstore Heval Hbody_replay_live Hbody_replay_consumed.
+  destruct Hsummary as [Hcaptured | Hdirect].
+  - eapply callee_body_root_shadow_captured_call_store_safe_summary_big_step_safe_checked_initial_ready;
+      eassumption.
+  - destruct (check_fn_root_shadow_direct_receiver_method_store_safe_summary_view_prop
+      env f Hdirect) as
+      (method_name & type_args & receiver_name & receiver_args & method_args &
+        target_synthetic_body & hidden_synthetic_body & receiver_callee &
+        method_callee & T_receiver & Gamma_receiver & R_receiver &
+        roots_receiver & T_receiver_env & Gamma_receiver_env & R_receiver_env &
+        roots_receiver_env & ret_roots_receiver & T_method & Gamma_method &
+        R_method & roots_method & T_method_env & Gamma_method_env &
+        R_method_env & roots_method_env & T_body & Gamma_body & R_out &
+        roots & _Htarget & _Hhidden & _Hsafe_receiver_args &
+        _Hsafe_method_args & _Hnot_free_method_args &
+        _Hnot_local_method_args & _Hnot_body_ctx & _Hin_receiver &
+        _Hname_receiver & _Hin_method & _Hname_method & _Harity & _Hbounds &
+        _Hreceiver_core & _Hreceiver_env & _Hreceiver_summary &
+        _Hreceiver_compat & _Hreceiver_roots & _Hreceiver_env_excl &
+        _Hmethod_core & _Hmethod_env & _Hmethod_ready & _Hmethod_summary &
+        _Hmethod_compat & _Hmethod_roots & _Hmethod_env_excl & Hbody_env &
+        _Hcompat & _Hroots_excl & _Henv_excl).
+    pose proof (infer_env_roots_shadow_safe_params_nodup_sidecar env
+      (fn_with_body f hidden_synthetic_body) (initial_root_env_for_fn f)
+      T_body Gamma_body R_out roots Hbody_env) as Hnodup.
+    unfold fn_with_body in Hnodup. simpl in Hnodup.
+    pose proof (initial_root_env_for_fn_no_shadow f Hnodup) as Hrn.
+    unfold direct_receiver_method_live_raw_body_replay_provider_for_eval
+      in Hbody_replay_live.
+    unfold direct_receiver_method_consumed_raw_body_replay_provider_for_eval
+      in Hbody_replay_consumed.
+    eapply callee_body_root_shadow_captured_call_direct_receiver_method_summary_runtime_replay_checked_initial_value_with_split_raw_body_replay;
+      try eassumption.
 Qed.
 
 Theorem env_root_shadow_captured_call_store_safe_or_no_capture_direct_component_summary_big_step_safe_checked_initial_ready_of_mutual :
